Impl/MarshallingModel.i.dfy
@@ -192,9 +192,13 @@ module MarshallingModel {
 
   function {:opaque} parseSector(data: seq<byte>) : (s : Option<Sector>)
   ensures s.Some? ==> SM.WFSector(s.value)
+  ensures s.Some? ==> Some(SM.ISector(s.value)) == Marshalling.parseSector(data)
+  ensures s.None? ==> Marshalling.parseSector(data).None?
   ensures s.Some? && s.value.SectorIndirectionTable? ==>
       IndirectionTableModel.TrackingGarbage(s.value.indirectionTable)
   {
+    Marshalling.reveal_parseSector();
+
     if |data| < 0x1_0000_0000_0000_0000 then (
       match parse_Val(data, Marshalling.SectorGrammar()).0 {
         case Some(v) => valToSector(v)
@@ -209,9 +213,13 @@ module MarshallingModel {
 
   function {:opaque} parseCheckedSector(data: seq<byte>) : (s : Option<Sector>)
   ensures s.Some? ==> SM.WFSector(s.value)
+  ensures s.Some? ==> Some(SM.ISector(s.value)) == Marshalling.parseCheckedSector(data)
+  ensures s.None? ==> Marshalling.parseCheckedSector(data).None?
   ensures s.Some? && s.value.SectorIndirectionTable? ==>
       IndirectionTableModel.TrackingGarbage(s.value.indirectionTable)
   {
+    Marshalling.reveal_parseCheckedSector();
+
     if |data| >= 32 && Crypto.Crc32C(data[32..]) == data[..32] then
       parseSector(data[32..])
     else
